trying to get to a compiling stage

pulse/lib/steel/pulse/Pulse.Checker.Admit.fst
@@ -10,64 +10,64 @@ open Pulse.Checker.Common
 
 module FV = Pulse.Typing.FV
 
-let post_hint_compatible (p:option post_hint_t) (x:var) (t:term) (u:universe) (post:vprop) =
-  match p with
-  | None -> True
-  | Some p ->
-    p.post== close_term post x /\
-    p.u == u /\
-    p.ret_ty == t
+// let post_hint_compatible (p:option post_hint_t) (x:var) (t:term) (u:universe) (post:vprop) =
+//   match p with
+//   | None -> True
+//   | Some p ->
+//     p.post== close_term post x /\
+//     p.u == u /\
+//     p.ret_ty == t
 
-#push-options "--z3rlimit_factor 4"
-let check_admit
-  (g:env)
-  (t:st_term{Tm_Admit? t.term})
-  (pre:term)
-  (pre_typing:tot_typing g pre tm_vprop)
-  (post_hint:post_hint_opt g)
-  (frame_pre:bool)
-  : T.Tac (checker_result_t g pre post_hint frame_pre) =
-  let Tm_Admit { ctag = c; typ=t; post } = t.term in
-  let x = fresh g in
-  let px = v_as_nv x in
-  let res
-    : (t:term &
-       u:universe &
-       universe_of g t u &
-       post:vprop { post_hint_compatible post_hint x t u post } &
-       tot_typing (push_binding g x (fst px) t) post tm_vprop)
-    = match post, post_hint with
-      | None, None
-      | Some _, Some _ ->
-        fail g None "T_Admit: either no post or two posts"
+// #push-options "--z3rlimit_factor 4"
+// let check_admit
+//   (g:env)
+//   (t:st_term{Tm_Admit? t.term})
+//   (pre:term)
+//   (pre_typing:tot_typing g pre tm_vprop)
+//   (post_hint:post_hint_opt g)
+//   (frame_pre:bool)
+//   : T.Tac (checker_result_t g pre post_hint frame_pre) =
+//   let Tm_Admit { ctag = c; typ=t; post } = t.term in
+//   let x = fresh g in
+//   let px = v_as_nv x in
+//   let res
+//     : (t:term &
+//        u:universe &
+//        universe_of g t u &
+//        post:vprop { post_hint_compatible post_hint x t u post } &
+//        tot_typing (push_binding g x (fst px) t) post tm_vprop)
+//     = match post, post_hint with
+//       | None, None
+//       | Some _, Some _ ->
+//         fail g None "T_Admit: either no post or two posts"
       
-      | Some post, _ ->
-        let (| u, t_typing |) = check_universe g t in    
-        let post_opened = open_term_nv post px in      
-        let (| post, post_typing |) = 
-            check_term_with_expected_type (push_binding g x (fst px) t) post_opened tm_vprop
-        in
-        (| t, u, t_typing, post, E post_typing |)
+//       | Some post, _ ->
+//         let (| u, t_typing |) = check_universe g t in    
+//         let post_opened = open_term_nv post px in      
+//         let (| post, post_typing |) = 
+//             check_term_with_expected_type (push_binding g x (fst px) t) post_opened tm_vprop
+//         in
+//         (| t, u, t_typing, post, E post_typing |)
 
-      | _, Some post ->
-        let post : post_hint_t = post in
-        if x `Set.mem` freevars post.post
-        then fail g None "Unexpected freevar clash in Tm_Admit"
-        else (
-          let post_typing_rec = post_hint_typing g post x in
-          let post_opened = open_term_nv post.post px in              
-          assume (close_term post_opened x == post.post);
-          (| post.ret_ty, post.u, post_typing_rec.ty_typing, post_opened, post_typing_rec.post_typing |)
-        )
-  in
-  let (| t, u, t_typing, post_opened, post_typing |) = res in
-  let post = close_term post_opened x in
-  let s : st_comp = {u;res=t;pre;post} in
+//       | _, Some post ->
+//         let post : post_hint_t = post in
+//         if x `Set.mem` freevars post.post
+//         then fail g None "Unexpected freevar clash in Tm_Admit"
+//         else (
+//           let post_typing_rec = post_hint_typing g post x in
+//           let post_opened = open_term_nv post.post px in              
+//           assume (close_term post_opened x == post.post);
+//           (| post.ret_ty, post.u, post_typing_rec.ty_typing, post_opened, post_typing_rec.post_typing |)
+//         )
+//   in
+//   let (| t, u, t_typing, post_opened, post_typing |) = res in
+//   let post = close_term post_opened x in
+//   let s : st_comp = {u;res=t;pre;post} in
 
-  assume (open_term (close_term post_opened x) x == post_opened);
-  (|
-     _, //Tm_Admit c u t None,
-     comp_admit c s,
-     T_Admit _ _ c (STC _ s x t_typing pre_typing post_typing)
-  |)
-#pop-options
+//   assume (open_term (close_term post_opened x) x == post_opened);
+//   (|
+//      _, //Tm_Admit c u t None,
+//      comp_admit c s,
+//      T_Admit _ _ c (STC _ s x t_typing pre_typing post_typing)
+//   |)
+// #pop-options
