pulse/lib/steel/pulse/Pulse.Checker.AssertWithBinders.fst
@@ -18,188 +18,188 @@ let is_host_term (t:R.term) = not (R.Tv_Unknown? (R.inspect_ln t))
 
 let debug_log = Pulse.Typing.debug_log "with_binders"
 
-let instantiate_binders_with_fresh_names (g:env) (top:R.term) : T.Tac (list nvar & R.term) =
-    let rec aux g (vars:list nvar) (t:R.term) : T.Tac (list nvar & R.term) = 
-        match R.inspect_ln t with
-        | R.Tv_Unknown -> T.fail "Impossible: instantiate_binders_with_fresh_names got an unknown term"
-        | R.Tv_Abs b body ->
-            let bv = R.inspect_binder b in
-            let x = fresh g in
-            let ppname = (mk_ppname bv.ppname (RU.range_of_term t)) in
-            let g = push_binding g x ppname (with_range Tm_Unknown (RU.range_of_term t)) in
-            let vars = (ppname, x)::vars in
-            let body = RT.open_term body x in
-            aux g vars body
-        | _ ->
-          L.rev vars, t
-    in
-    aux g [] top
+// let instantiate_binders_with_fresh_names (g:env) (top:R.term) : T.Tac (list nvar & R.term) =
+//     let rec aux g (vars:list nvar) (t:R.term) : T.Tac (list nvar & R.term) = 
+//         match R.inspect_ln t with
+//         | R.Tv_Unknown -> T.fail "Impossible: instantiate_binders_with_fresh_names got an unknown term"
+//         | R.Tv_Abs b body ->
+//             let bv = R.inspect_binder b in
+//             let x = fresh g in
+//             let ppname = (mk_ppname bv.ppname (RU.range_of_term t)) in
+//             let g = push_binding g x ppname (with_range Tm_Unknown (RU.range_of_term t)) in
+//             let vars = (ppname, x)::vars in
+//             let body = RT.open_term body x in
+//             aux g vars body
+//         | _ ->
+//           L.rev vars, t
+//     in
+//     aux g [] top
 
-let instantiate_names_with_uvars (xs:list nvar) (t0 t1:term)
-  : T.Tac (list (Inf.uvar & term) & vprop & vprop)
-  = let subst, out =
-      T.fold_right (fun (p,x) (subst, out) ->
-        let uv, t = Inf.gen_uvar p in
-        let out = (uv, t)::out in
-        let subst = N.NT x t :: subst in
-        subst, out)
-        xs
-        ([], [])
-    in
-    out, subst_term t0 subst, subst_term t1 subst
+// let instantiate_names_with_uvars (xs:list nvar) (t0 t1:term)
+//   : T.Tac (list (Inf.uvar & term) & vprop & vprop)
+//   = let subst, out =
+//       T.fold_right (fun (p,x) (subst, out) ->
+//         let uv, t = Inf.gen_uvar p in
+//         let out = (uv, t)::out in
+//         let subst = N.NT x t :: subst in
+//         subst, out)
+//         xs
+//         ([], [])
+//     in
+//     out, subst_term t0 subst, subst_term t1 subst
 
-let instantiate_binders_with_uvars (top:R.term) : T.Tac (list (Inf.uvar & term) & vprop) =
-    let rec aux uvars (t:R.term) : T.Tac (list (Inf.uvar & term) & vprop) = 
-        match R.inspect_ln t with
-        | R.Tv_Unknown -> T.fail "Impossible: instantiate_binders_with_uvars got an unknown term"
-        | R.Tv_Abs b body ->
-            let bv = R.inspect_binder b in
-            let uv, t = Inf.gen_uvar (mk_ppname bv.ppname (RU.range_of_term t)) in
-            let uvars = (uv, t)::uvars in
-            let body = RT.subst_term body N.(rt_subst [DT 0 t]) in
-            aux uvars body
-        | _ ->
-          match readback_ty t with
-          | None -> T.fail "Failed to readback elaborated assertion"
-          | Some t -> L.rev uvars, t
-    in
-    aux [] top
+// let instantiate_binders_with_uvars (top:R.term) : T.Tac (list (Inf.uvar & term) & vprop) =
+//     let rec aux uvars (t:R.term) : T.Tac (list (Inf.uvar & term) & vprop) = 
+//         match R.inspect_ln t with
+//         | R.Tv_Unknown -> T.fail "Impossible: instantiate_binders_with_uvars got an unknown term"
+//         | R.Tv_Abs b body ->
+//             let bv = R.inspect_binder b in
+//             let uv, t = Inf.gen_uvar (mk_ppname bv.ppname (RU.range_of_term t)) in
+//             let uvars = (uv, t)::uvars in
+//             let body = RT.subst_term body N.(rt_subst [DT 0 t]) in
+//             aux uvars body
+//         | _ ->
+//           match readback_ty t with
+//           | None -> T.fail "Failed to readback elaborated assertion"
+//           | Some t -> L.rev uvars, t
+//     in
+//     aux [] top
 
-let infer_binder_types (g:env) (bs:list binder) (v:vprop)
-  : T.Tac (list nvar & R.term) = 
-    let tv = elab_term v in
-    if not (is_host_term tv)
-    then fail g (Some v.range) (Printf.sprintf "Cannot infer type of %s" (P.term_to_string v));
-    let as_binder (b:binder) : R.binder =
-        let open R in
-        let bv : binder_view = 
-            { sort = elab_term b.binder_ty;
-              ppname = b.binder_ppname.name;
-              qual = Q_Explicit;
-              attrs = [] } in
-        pack_binder bv
-    in
-    let abstraction = 
-        L.fold_right 
-            (fun b (tv:host_term) -> 
-                let b = as_binder b in
-                R.pack_ln (R.Tv_Abs b tv))
-            bs
-            tv
-    in
-    // T.print (Printf.sprintf "About to elaborate assert body: %s" (T.term_to_string abstraction));
-    let inst_abstraction, _ = PC.instantiate_term_implicits g (tm_fstar abstraction v.range) in
-    // T.print (Printf.sprintf "Instantiated abstraction is: %s" (T.term_to_string abstraction));
-    match inst_abstraction.t with
-    | Tm_FStar t -> instantiate_binders_with_fresh_names g t
-    | t ->
-      match bs with
-      | [] -> [], elab_term inst_abstraction
-      | _ -> T.fail "Impossible: Instantiated abstraction is not embedded F* term"
+// let infer_binder_types (g:env) (bs:list binder) (v:vprop)
+//   : T.Tac (list nvar & R.term) = 
+//     let tv = elab_term v in
+//     if not (is_host_term tv)
+//     then fail g (Some v.range) (Printf.sprintf "Cannot infer type of %s" (P.term_to_string v));
+//     let as_binder (b:binder) : R.binder =
+//         let open R in
+//         let bv : binder_view = 
+//             { sort = elab_term b.binder_ty;
+//               ppname = b.binder_ppname.name;
+//               qual = Q_Explicit;
+//               attrs = [] } in
+//         pack_binder bv
+//     in
+//     let abstraction = 
+//         L.fold_right 
+//             (fun b (tv:host_term) -> 
+//                 let b = as_binder b in
+//                 R.pack_ln (R.Tv_Abs b tv))
+//             bs
+//             tv
+//     in
+//     // T.print (Printf.sprintf "About to elaborate assert body: %s" (T.term_to_string abstraction));
+//     let inst_abstraction, _ = PC.instantiate_term_implicits g (tm_fstar abstraction v.range) in
+//     // T.print (Printf.sprintf "Instantiated abstraction is: %s" (T.term_to_string abstraction));
+//     match inst_abstraction.t with
+//     | Tm_FStar t -> instantiate_binders_with_fresh_names g t
+//     | t ->
+//       match bs with
+//       | [] -> [], elab_term inst_abstraction
+//       | _ -> T.fail "Impossible: Instantiated abstraction is not embedded F* term"
 
-let option_must (f:option 'a) (msg:string) : T.Tac 'a =
-  match f with
-  | Some x -> x
-  | None -> T.fail msg
+// let option_must (f:option 'a) (msg:string) : T.Tac 'a =
+//   match f with
+//   | Some x -> x
+//   | None -> T.fail msg
 
-let unfold_defs (g:env) (defs:option (list string)) (t:R.term) 
-  : T.Tac term
-  = let head, _ = T.collect_app t in
-    match R.inspect_ln head with
-    | R.Tv_FVar fv
-    | R.Tv_UInst fv _ -> (
-        let head = String.concat "." (R.inspect_fv fv) in
-        let fully = 
-          match defs with
-          | Some defs -> defs
-          | None -> []
-        in
-        let rt = RU.unfold_def (fstar_env g) head fully t in
-        let rt = option_must rt "Unexpected: reduction produced an ill-formed term" in
-        let ty = option_must (readback_ty rt) "Unexpected: unable to readback unfolded term" in
-        debug_log g (fun _ -> Printf.sprintf "Unfolded %s to F* term %s and readback as %s" (T.term_to_string t) (T.term_to_string rt) (P.term_to_string ty));
-        ty
-      )
-    | _ ->
-      fail g (Some (RU.range_of_term t)) (Printf.sprintf "Cannot unfold %s" (T.term_to_string t))
+// let unfold_defs (g:env) (defs:option (list string)) (t:R.term) 
+//   : T.Tac term
+//   = let head, _ = T.collect_app t in
+//     match R.inspect_ln head with
+//     | R.Tv_FVar fv
+//     | R.Tv_UInst fv _ -> (
+//         let head = String.concat "." (R.inspect_fv fv) in
+//         let fully = 
+//           match defs with
+//           | Some defs -> defs
+//           | None -> []
+//         in
+//         let rt = RU.unfold_def (fstar_env g) head fully t in
+//         let rt = option_must rt "Unexpected: reduction produced an ill-formed term" in
+//         let ty = option_must (readback_ty rt) "Unexpected: unable to readback unfolded term" in
+//         debug_log g (fun _ -> Printf.sprintf "Unfolded %s to F* term %s and readback as %s" (T.term_to_string t) (T.term_to_string rt) (P.term_to_string ty));
+//         ty
+//       )
+//     | _ ->
+//       fail g (Some (RU.range_of_term t)) (Printf.sprintf "Cannot unfold %s" (T.term_to_string t))
     
-let prepare_goal hint_type g (v:R.term) : T.Tac (term & term) = 
-  match hint_type with
-  | ASSERT -> 
-    let v = option_must (readback_ty v) "Failed to readback elaborated assertion" in
-    v, v
-  | UNFOLD _ -> 
-    option_must (readback_ty v) "Failed to readback elaborated assertion",
-    unfold_defs g None v
-  | FOLD ns -> 
-    unfold_defs g ns v,
-    option_must (readback_ty v) "Failed to readback elaborated assertion"
+// let prepare_goal hint_type g (v:R.term) : T.Tac (term & term) = 
+//   match hint_type with
+//   | ASSERT -> 
+//     let v = option_must (readback_ty v) "Failed to readback elaborated assertion" in
+//     v, v
+//   | UNFOLD _ -> 
+//     option_must (readback_ty v) "Failed to readback elaborated assertion",
+//     unfold_defs g None v
+//   | FOLD ns -> 
+//     unfold_defs g ns v,
+//     option_must (readback_ty v) "Failed to readback elaborated assertion"
 
-let check_unfoldable g hint_type (v:term) : T.Tac unit = 
-  match hint_type with
-  | ASSERT -> ()
-  | FOLD _ 
-  | UNFOLD _ ->
-    match v.t with
-    | Tm_FStar _ -> ()
-    | _ -> 
-     fail g 
-        (Some v.range)
-        (Printf.sprintf "`fold` and `unfold` expect a single user-defined predicate as an argument, \
-                          but %s is a primitive term that cannot be folded or unfolded"
-                          (P.term_to_string v))
+// let check_unfoldable g hint_type (v:term) : T.Tac unit = 
+//   match hint_type with
+//   | ASSERT -> ()
+//   | FOLD _ 
+//   | UNFOLD _ ->
+//     match v.t with
+//     | Tm_FStar _ -> ()
+//     | _ -> 
+//      fail g 
+//         (Some v.range)
+//         (Printf.sprintf "`fold` and `unfold` expect a single user-defined predicate as an argument, \
+//                           but %s is a primitive term that cannot be folded or unfolded"
+//                           (P.term_to_string v))
 
-let check
-  (g:env)
-  (st:st_term{Tm_ProofHintWithBinders? st.term})
-  (pre:term)
-  (pre_typing:tot_typing g pre tm_vprop)
-  (post_hint:post_hint_opt g)
-  (frame_pre:bool)
-  (check:check_t)
-  : T.Tac (checker_result_t g pre post_hint frame_pre)
-  = let Tm_ProofHintWithBinders { hint_type; binders; v; t=body } = st.term in
-    check_unfoldable g hint_type v;
-    let nvars, v = infer_binder_types g binders v in
-    let lhs, rhs = prepare_goal hint_type g v in
-    let uvs, lhs, rhs = instantiate_names_with_uvars nvars lhs rhs in
-    debug_log g (fun _ -> Printf.sprintf "Trying to solve %s \nagainst context %s" (P.term_to_string lhs) (P.term_to_string pre));
-    let solution = Pulse.Checker.Inference.try_inst_uvs_in_goal g pre lhs in
-    match Inf.unsolved solution uvs with
-    | Some uvs ->
-      fail g (Some st.range) 
-             (Printf.sprintf "Could not instantiate %s"
-                             (String.concat ", " (T.map (fun (_, t) -> P.term_to_string t) uvs)))
-    | _ ->
-      debug_log g (fun _ -> Printf.sprintf "Solution: %s\n" (Inf.solutions_to_string solution));
-      let sub = 
-        T.fold_left 
-            (fun subst (uv, t) ->
-                let sol = Inf.apply_solution solution t in 
-                N.DT 0 sol::shift_subst subst)
-            []
-            uvs
-      in
-      let seq t1 t2 = 
-          { term = Tm_Bind { binder = as_binder (tm_fstar (`unit) st.range);
-                             head = t1; body = t2 };
-            range = st.range }
-      in
-      match hint_type with
-      | ASSERT ->
-        let assert_term = tm_fstar (`(Pulse.Steel.Wrapper.assert_)) st.range in
-        let vprop_to_assert = Inf.apply_solution solution lhs in
-        let asrt = { term = Tm_STApp { head=assert_term; arg_qual=None; arg=vprop_to_assert}; 
-                     range = st.range } in
-        let tm = seq asrt (subst_st_term body sub) in
-        debug_log g (fun _ -> Printf.sprintf "After with_binders: about to check %s\n" (P.st_term_to_string tm));
-        check g tm pre pre_typing post_hint frame_pre
-      | UNFOLD _
-      | FOLD _ ->
-        let rw = { term = Tm_Rewrite { t1 = Inf.apply_solution solution lhs;
-                                       t2 = Inf.apply_solution solution rhs };
-                   range = st.range } in
-        let body' = subst_st_term body sub in
-        let tm = seq rw body' in
-        debug_log g (fun _ -> Printf.sprintf "After with_binders: about to check %s\n" (P.st_term_to_string tm));
-        check g tm pre pre_typing post_hint frame_pre
+// let check
+//   (g:env)
+//   (st:st_term{Tm_ProofHintWithBinders? st.term})
+//   (pre:term)
+//   (pre_typing:tot_typing g pre tm_vprop)
+//   (post_hint:post_hint_opt g)
+//   (frame_pre:bool)
+//   (check:check_t)
+//   : T.Tac (checker_result_t g pre post_hint frame_pre)
+//   = let Tm_ProofHintWithBinders { hint_type; binders; v; t=body } = st.term in
+//     check_unfoldable g hint_type v;
+//     let nvars, v = infer_binder_types g binders v in
+//     let lhs, rhs = prepare_goal hint_type g v in
+//     let uvs, lhs, rhs = instantiate_names_with_uvars nvars lhs rhs in
+//     debug_log g (fun _ -> Printf.sprintf "Trying to solve %s \nagainst context %s" (P.term_to_string lhs) (P.term_to_string pre));
+//     let solution = Pulse.Checker.Inference.try_inst_uvs_in_goal g pre lhs in
+//     match Inf.unsolved solution uvs with
+//     | Some uvs ->
+//       fail g (Some st.range) 
+//              (Printf.sprintf "Could not instantiate %s"
+//                              (String.concat ", " (T.map (fun (_, t) -> P.term_to_string t) uvs)))
+//     | _ ->
+//       debug_log g (fun _ -> Printf.sprintf "Solution: %s\n" (Inf.solutions_to_string solution));
+//       let sub = 
+//         T.fold_left 
+//             (fun subst (uv, t) ->
+//                 let sol = Inf.apply_solution solution t in 
+//                 N.DT 0 sol::shift_subst subst)
+//             []
+//             uvs
+//       in
+//       let seq t1 t2 = 
+//           { term = Tm_Bind { binder = as_binder (tm_fstar (`unit) st.range);
+//                              head = t1; body = t2 };
+//             range = st.range }
+//       in
+//       match hint_type with
+//       | ASSERT ->
+//         let assert_term = tm_fstar (`(Pulse.Steel.Wrapper.assert_)) st.range in
+//         let vprop_to_assert = Inf.apply_solution solution lhs in
+//         let asrt = { term = Tm_STApp { head=assert_term; arg_qual=None; arg=vprop_to_assert}; 
+//                      range = st.range } in
+//         let tm = seq asrt (subst_st_term body sub) in
+//         debug_log g (fun _ -> Printf.sprintf "After with_binders: about to check %s\n" (P.st_term_to_string tm));
+//         check g tm pre pre_typing post_hint frame_pre
+//       | UNFOLD _
+//       | FOLD _ ->
+//         let rw = { term = Tm_Rewrite { t1 = Inf.apply_solution solution lhs;
+//                                        t2 = Inf.apply_solution solution rhs };
+//                    range = st.range } in
+//         let body' = subst_st_term body sub in
+//         let tm = seq rw body' in
+//         debug_log g (fun _ -> Printf.sprintf "After with_binders: about to check %s\n" (P.st_term_to_string tm));
+//         check g tm pre pre_typing post_hint frame_pre
