pulse/lib/steel/pulse/Pulse.Checker.WithLocal.fst
@@ -10,82 +10,82 @@ open Pulse.Checker.Common
 
 module FV = Pulse.Typing.FV
 
-#push-options "--z3rlimit_factor 4"
-let extend_post_hint_for_local (g:env) (p:post_hint_for_env g)
-                               (init_t:term) (x:var { ~ (Set.mem x (dom g)) })
-  : post_hint_for_env (push_binding g x ppname_default init_t)
-  = { p with post = comp_withlocal_body_post p.post init_t (null_var x);
-             post_typing = admit() } //star typing intro
+// #push-options "--z3rlimit_factor 4"
+// let extend_post_hint_for_local (g:env) (p:post_hint_for_env g)
+//                                (init_t:term) (x:var { ~ (Set.mem x (dom g)) })
+//   : post_hint_for_env (push_binding g x ppname_default init_t)
+//   = { p with post = comp_withlocal_body_post p.post init_t (null_var x);
+//              post_typing = admit() } //star typing intro
 
-let with_local_pre_typing (#g:env) (#pre:term) (pre_typing:tot_typing g pre tm_vprop)
-                          (init_t:term) (x:var { ~ (Set.mem x (dom g)) }) (i:term)
-  : tot_typing (push_binding g x ppname_default (mk_ref init_t))
-               (comp_withlocal_body_pre pre init_t (null_var x) i)
-               tm_vprop
-  = admit()
+// let with_local_pre_typing (#g:env) (#pre:term) (pre_typing:tot_typing g pre tm_vprop)
+//                           (init_t:term) (x:var { ~ (Set.mem x (dom g)) }) (i:term)
+//   : tot_typing (push_binding g x ppname_default (mk_ref init_t))
+//                (comp_withlocal_body_pre pre init_t (null_var x) i)
+//                tm_vprop
+//   = admit()
 
 
   
-let check_withlocal
-  (allow_inst:bool)
-  (g:env)
-  (t:st_term{Tm_WithLocal? t.term})
-  (pre:term)
-  (pre_typing:tot_typing g pre tm_vprop)
-  (post_hint:post_hint_opt g)
-  (frame_pre:bool)
-  (check':bool -> check_t)
-  : T.Tac (checker_result_t g pre post_hint frame_pre) =
-  if not frame_pre
-  then T.fail "withlocal: frame_pre is false, bailing";
-  let g = push_context "check_withlocal" t.range g in
-  let wr t0 = { term = t0; range = t.range } in
-  let Tm_WithLocal {binder; initializer=init; body} = t.term in
-  let (| init, init_u, init_t, init_t_typing, init_typing |) =
-    check_term_and_type g init in
-  if eq_univ init_u u0
-  then let x = fresh g in
-       let px = binder.binder_ppname, x in
-       if x `Set.mem` freevars_st body
-       then fail g (Some body.range) (Printf.sprintf "withlocal: %s is free in body" (T.unseal binder.binder_ppname.name))
-       else
-         let x_tm = term_of_nvar px in
-         let g_extended = push_binding g x binder.binder_ppname (mk_ref init_t) in
-         let body_pre = comp_withlocal_body_pre pre init_t x_tm init in
-         let body_pre_typing = with_local_pre_typing pre_typing init_t x init in
-         // elaborating this post here,
-         //   so that later we can check the computed post to be equal to this one
-         let post : post_hint_for_env g =
-           // let post =
-             match post_hint with
-             | Some post -> post
-             | None -> fail g None "Allocating a mutable local variable expects an annotated post-condition"
-         in
-         if x `Set.mem` freevars post.post
-         then fail g None "Unexpected name clash in with_local"
-         else (
-           let body_post = extend_post_hint_for_local g post init_t x in
-           let (| opened_body, c_body, body_typing |) =
-             check' allow_inst g_extended (open_st_term_nv body px) body_pre body_pre_typing (Some body_post) frame_pre in
-           //
-           // Checking post equality here to match the typing rule
-           // 
-           if not (C_ST? c_body)
-           then fail g (Some body.range) "withlocal: body is not stt or postcondition mismatch"
-           else let body = close_st_term opened_body x in
-                assume (open_st_term (close_st_term opened_body x) x == opened_body);
-                let c = C_ST {u=comp_u c_body;res=comp_res c_body;pre;post=post.post} in
-                let c_typing =
-                    let post_typing_rec = post_hint_typing g post x in
-                    intro_comp_typing g c pre_typing post_typing_rec.ty_typing x post_typing_rec.post_typing
-                in
-                let d = T_WithLocal g init body init_t c x
-                                    (E init_typing)
-                                    init_t_typing
-                                    c_typing
-                                    body_typing 
-                in
-                (| _, _, d |)
-         )
-  else fail g None "Allocating a local variable: init type is not universe zero"
-#pop-options
+// let check_withlocal
+//   (allow_inst:bool)
+//   (g:env)
+//   (t:st_term{Tm_WithLocal? t.term})
+//   (pre:term)
+//   (pre_typing:tot_typing g pre tm_vprop)
+//   (post_hint:post_hint_opt g)
+//   (frame_pre:bool)
+//   (check':bool -> check_t)
+//   : T.Tac (checker_result_t g pre post_hint frame_pre) =
+//   if not frame_pre
+//   then T.fail "withlocal: frame_pre is false, bailing";
+//   let g = push_context "check_withlocal" t.range g in
+//   let wr t0 = { term = t0; range = t.range } in
+//   let Tm_WithLocal {binder; initializer=init; body} = t.term in
+//   let (| init, init_u, init_t, init_t_typing, init_typing |) =
+//     check_term_and_type g init in
+//   if eq_univ init_u u0
+//   then let x = fresh g in
+//        let px = binder.binder_ppname, x in
+//        if x `Set.mem` freevars_st body
+//        then fail g (Some body.range) (Printf.sprintf "withlocal: %s is free in body" (T.unseal binder.binder_ppname.name))
+//        else
+//          let x_tm = term_of_nvar px in
+//          let g_extended = push_binding g x binder.binder_ppname (mk_ref init_t) in
+//          let body_pre = comp_withlocal_body_pre pre init_t x_tm init in
+//          let body_pre_typing = with_local_pre_typing pre_typing init_t x init in
+//          // elaborating this post here,
+//          //   so that later we can check the computed post to be equal to this one
+//          let post : post_hint_for_env g =
+//            // let post =
+//              match post_hint with
+//              | Some post -> post
+//              | None -> fail g None "Allocating a mutable local variable expects an annotated post-condition"
+//          in
+//          if x `Set.mem` freevars post.post
+//          then fail g None "Unexpected name clash in with_local"
+//          else (
+//            let body_post = extend_post_hint_for_local g post init_t x in
+//            let (| opened_body, c_body, body_typing |) =
+//              check' allow_inst g_extended (open_st_term_nv body px) body_pre body_pre_typing (Some body_post) frame_pre in
+//            //
+//            // Checking post equality here to match the typing rule
+//            // 
+//            if not (C_ST? c_body)
+//            then fail g (Some body.range) "withlocal: body is not stt or postcondition mismatch"
+//            else let body = close_st_term opened_body x in
+//                 assume (open_st_term (close_st_term opened_body x) x == opened_body);
+//                 let c = C_ST {u=comp_u c_body;res=comp_res c_body;pre;post=post.post} in
+//                 let c_typing =
+//                     let post_typing_rec = post_hint_typing g post x in
+//                     intro_comp_typing g c pre_typing post_typing_rec.ty_typing x post_typing_rec.post_typing
+//                 in
+//                 let d = T_WithLocal g init body init_t c x
+//                                     (E init_typing)
+//                                     init_t_typing
+//                                     c_typing
+//                                     body_typing 
+//                 in
+//                 (| _, _, d |)
+//          )
+//   else fail g None "Allocating a local variable: init type is not universe zero"
+// #pop-options
