pulse/lib/steel/pulse/Pulse.Checker.Abs.fst
@@ -37,13 +37,13 @@ let check_abs
   (pre:term)
   (pre_typing:tot_typing g pre tm_vprop)
   (post_hint:post_hint_opt g)
-  (frame_pre:bool)
   (check:check_t)
-  : T.Tac (checker_result_t g pre post_hint frame_pre) =
+  : T.Tac (checker_result_t g pre post_hint) =
   if Some? post_hint then fail g None "Unexpected post-condition annotation from context for an abstraction" else 
   let range = t.range in
   match t.term with  
   | Tm_Abs { b = {binder_ty=t;binder_ppname=ppname}; q=qual; ascription=c; body } -> //pre=pre_hint; body; ret_ty; post=post_hint_body } ->
+
     (*  (fun (x:t) -> {pre_hint} body : t { post_hint } *)
     let (| t, _, _ |) = check_term g t in //elaborate it first
     let (| u, t_typing |) = check_universe g t in //then check that its universe ... We could collapse the two calls
@@ -78,12 +78,16 @@ let check_abs
         in
         Some post_hint_typing
     in
-    let (| body', c_body, body_typing |) = check g' (open_st_term_nv body px) pre_opened pre_typing post frame_pre in
-    check_effect_annotation g' body'.range c c_body;
-    FV.st_typing_freevars body_typing;
-    let body_closed = close_st_term body' x in
-    assume (open_st_term body_closed x == body');
-    let b = {binder_ty=t;binder_ppname=ppname} in
-    let tt = T_Abs g x qual b u body_closed c_body t_typing body_typing in
-    let tres = tm_arrow {binder_ty=t;binder_ppname=ppname} qual (close_comp c_body x) in
-    (| _, C_Tot tres, tt |)
+
+
+    admit ()
+
+    // let (| body', c_body, body_typing |) = check g' (open_st_term_nv body px) pre_opened pre_typing post frame_pre in
+    // check_effect_annotation g' body'.range c c_body;
+    // FV.st_typing_freevars body_typing;
+    // let body_closed = close_st_term body' x in
+    // assume (open_st_term body_closed x == body');
+    // let b = {binder_ty=t;binder_ppname=ppname} in
+    // let tt = T_Abs g x qual b u body_closed c_body t_typing body_typing in
+    // let tres = tm_arrow {binder_ty=t;binder_ppname=ppname} qual (close_comp c_body x) in
+    // (| _, C_Tot tres, tt |)
