pulse/lib/steel/pulse/Pulse.Checker.Exists.fsti
@@ -6,30 +6,30 @@ open Pulse.Syntax
 open Pulse.Typing
 open Pulse.Checker.Common
 
-val check_elim_exists
-  (g:env)
-  (t:st_term{Tm_ElimExists? t.term})
-  (pre:term)
-  (pre_typing:tot_typing g pre tm_vprop)
-  (post_hint:post_hint_opt g)
-  (frame_pre:bool)
-  : T.Tac (checker_result_t g pre post_hint frame_pre)
+// val check_elim_exists
+//   (g:env)
+//   (t:st_term{Tm_ElimExists? t.term})
+//   (pre:term)
+//   (pre_typing:tot_typing g pre tm_vprop)
+//   (post_hint:post_hint_opt g)
+//   (frame_pre:bool)
+//   : T.Tac (checker_result_t g pre post_hint frame_pre)
 
-let intro_exists_witness_singleton (st:st_term)  = 
-  match st.term with
-  | Tm_IntroExists { witnesses = [_] } -> true
-  | _ -> false
+// let intro_exists_witness_singleton (st:st_term)  = 
+//   match st.term with
+//   | Tm_IntroExists { witnesses = [_] } -> true
+//   | _ -> false
 
-let intro_exists_vprop (st:st_term { Tm_IntroExists? st.term })  = 
-  match st.term with
-  | Tm_IntroExists { p } -> p
+// let intro_exists_vprop (st:st_term { Tm_IntroExists? st.term })  = 
+//   match st.term with
+//   | Tm_IntroExists { p } -> p
 
-val check_intro_exists_either
-  (g:env)
-  (st:st_term{intro_exists_witness_singleton st})
-  (vprop_typing: option (tot_typing g (intro_exists_vprop st) tm_vprop))
-  (pre:term)
-  (pre_typing:tot_typing g pre tm_vprop)
-  (post_hint:post_hint_opt g)
-  (frame_pre:bool)
-  : T.Tac (checker_result_t g pre post_hint frame_pre)
+// val check_intro_exists_either
+//   (g:env)
+//   (st:st_term{intro_exists_witness_singleton st})
+//   (vprop_typing: option (tot_typing g (intro_exists_vprop st) tm_vprop))
+//   (pre:term)
+//   (pre_typing:tot_typing g pre tm_vprop)
+//   (post_hint:post_hint_opt g)
+//   (frame_pre:bool)
+//   : T.Tac (checker_result_t g pre post_hint frame_pre)
