pulse/lib/steel/pulse/Pulse.Checker.If.fsti
@@ -6,13 +6,13 @@ open Pulse.Syntax
 open Pulse.Typing
 open Pulse.Checker.Common
 
-val check_if
-  (g:env)
-  (b:term)
-  (e1 e2:st_term)
-  (pre:term)
-  (pre_typing: tot_typing g pre tm_vprop)
-  (post_hint:post_hint_for_env g)
-  (frame_pre:bool)
-  (check:check_t)
-  : T.Tac (checker_result_t g pre (Some post_hint) frame_pre)
+// val check_if
+//   (g:env)
+//   (b:term)
+//   (e1 e2:st_term)
+//   (pre:term)
+//   (pre_typing: tot_typing g pre tm_vprop)
+//   (post_hint:post_hint_for_env g)
+//   (frame_pre:bool)
+//   (check:check_t)
+//   : T.Tac (checker_result_t g pre (Some post_hint) frame_pre)
