pulse/lib/steel/pulse/Pulse.Checker.Return.fsti
@@ -6,12 +6,12 @@ open Pulse.Syntax
 open Pulse.Typing
 open Pulse.Checker.Common
 
-val check_return
-  (allow_inst:bool)
-  (g:env)
-  (st:st_term{Tm_Return? st.term})
-  (pre:term)
-  (pre_typing:tot_typing g pre tm_vprop)
-  (post_hint:post_hint_opt g)
-  (frame_pre:bool)
-  : T.Tac (checker_result_t g pre post_hint frame_pre)
+// val check_return
+//   (allow_inst:bool)
+//   (g:env)
+//   (st:st_term{Tm_Return? st.term})
+//   (pre:term)
+//   (pre_typing:tot_typing g pre tm_vprop)
+//   (post_hint:post_hint_opt g)
+//   (frame_pre:bool)
+//   : T.Tac (checker_result_t g pre post_hint frame_pre)
