pulse/lib/steel/pulse/Pulse.Checker.Rewrite.fst
@@ -10,38 +10,38 @@ open Pulse.Checker.Common
 module P = Pulse.Syntax.Printer
 module FV = Pulse.Typing.FV
 
-let check_rewrite
-  (g:env)
-  (t:st_term{Tm_Rewrite? t.term})
-  (pre:term)
-  (pre_typing:tot_typing g pre tm_vprop)
-  (post_hint:post_hint_opt g)
-  (frame_pre:bool)
-  : T.Tac (checker_result_t g pre post_hint frame_pre) =
-  let g = push_context "check_rewrite" t.range g in
-  let Tm_Rewrite {t1=p; t2=q} = t.term in
-  let (| p, p_typing |) = check_vprop g p in
-  let (| q, q_typing |) = check_vprop g q in
-  let equiv_p_q =
-      if eq_tm p q
-      then VE_Refl g p
-      else let elab_p = elab_term p in
-           let elab_q = elab_term q in
-           let res, issues = T.check_equiv (elab_env g) elab_p elab_q in
-           T.log_issues issues;
-           match res with
-           | None -> 
-             fail g (Some t.range)
-                    (Printf.sprintf "rewrite: could not prove equality of %s and %s\nElaborations: %s and %s\n" 
-                           (P.term_to_string p)
-                           (P.term_to_string q)
-                           (T.term_to_string elab_p)
-                           (T.term_to_string elab_q))
-           | Some token ->
-            VE_Ext g p q token in
-	let d = T_Rewrite _ p q p_typing equiv_p_q in
-  if frame_pre
-	then repack (Pulse.Checker.Common.try_frame_pre pre_typing d) post_hint
-  else if Some? post_hint
-  then T.fail "check_rewrite: frame_pre is false but post_hint is set, bailing"
-  else (| _, _, d |)
+// let check_rewrite
+//   (g:env)
+//   (t:st_term{Tm_Rewrite? t.term})
+//   (pre:term)
+//   (pre_typing:tot_typing g pre tm_vprop)
+//   (post_hint:post_hint_opt g)
+//   (frame_pre:bool)
+//   : T.Tac (checker_result_t g pre post_hint frame_pre) =
+//   let g = push_context "check_rewrite" t.range g in
+//   let Tm_Rewrite {t1=p; t2=q} = t.term in
+//   let (| p, p_typing |) = check_vprop g p in
+//   let (| q, q_typing |) = check_vprop g q in
+//   let equiv_p_q =
+//       if eq_tm p q
+//       then VE_Refl g p
+//       else let elab_p = elab_term p in
+//            let elab_q = elab_term q in
+//            let res, issues = T.check_equiv (elab_env g) elab_p elab_q in
+//            T.log_issues issues;
+//            match res with
+//            | None -> 
+//              fail g (Some t.range)
+//                     (Printf.sprintf "rewrite: could not prove equality of %s and %s\nElaborations: %s and %s\n" 
+//                            (P.term_to_string p)
+//                            (P.term_to_string q)
+//                            (T.term_to_string elab_p)
+//                            (T.term_to_string elab_q))
+//            | Some token ->
+//             VE_Ext g p q token in
+// 	let d = T_Rewrite _ p q p_typing equiv_p_q in
+//   if frame_pre
+// 	then repack (Pulse.Checker.Common.try_frame_pre pre_typing d) post_hint
+//   else if Some? post_hint
+//   then T.fail "check_rewrite: frame_pre is false but post_hint is set, bailing"
+//   else (| _, _, d |)
