pulse/lib/steel/pulse/Pulse.Checker.While.fst
@@ -14,101 +14,101 @@ module Framing = Pulse.Checker.Framing
 module Metatheory = Pulse.Typing.Metatheory
 module RU = Pulse.RuntimeUtils
 
-let while_cond_comp_typing (#g:env) (u:universe) (x:ppname) (ty:term) (inv_body:term)
-                           (inv_typing:tot_typing g (tm_exists_sl u (as_binder ty) inv_body) tm_vprop)
-  : Metatheory.comp_typing_u g (comp_while_cond x inv_body)
-  = Metatheory.admit_comp_typing g (comp_while_cond x inv_body)
+// let while_cond_comp_typing (#g:env) (u:universe) (x:ppname) (ty:term) (inv_body:term)
+//                            (inv_typing:tot_typing g (tm_exists_sl u (as_binder ty) inv_body) tm_vprop)
+//   : Metatheory.comp_typing_u g (comp_while_cond x inv_body)
+//   = Metatheory.admit_comp_typing g (comp_while_cond x inv_body)
 
-let while_body_comp_typing (#g:env) (u:universe) (x:ppname) (ty:term) (inv_body:term)
-                           (inv_typing:tot_typing g (tm_exists_sl u (as_binder ty) inv_body) tm_vprop)
-  : Metatheory.comp_typing_u g (comp_while_body x inv_body)
-  = Metatheory.admit_comp_typing g (comp_while_body x inv_body)
+// let while_body_comp_typing (#g:env) (u:universe) (x:ppname) (ty:term) (inv_body:term)
+//                            (inv_typing:tot_typing g (tm_exists_sl u (as_binder ty) inv_body) tm_vprop)
+//   : Metatheory.comp_typing_u g (comp_while_body x inv_body)
+//   = Metatheory.admit_comp_typing g (comp_while_body x inv_body)
 
-#push-options "--fuel 0 --ifuel 2 --z3rlimit_factor 10 --split_queries no --query_stats"
-let check_while
-  (allow_inst:bool)
-  (g:env)
-  (t:st_term{Tm_While? t.term})
-  (pre:term)
-  (pre_typing:tot_typing g pre tm_vprop)
-  (post_hint:post_hint_opt g)
-  (frame_pre:bool)
-  (check':bool -> check_t)
-  : T.Tac (checker_result_t g pre post_hint frame_pre) =
-  if not frame_pre
-  then T.fail "check_while, frame_pre is false, bailing";
-  let g = push_context "while loop" t.range g in
-  let Tm_While { invariant=inv; condition=cond; body; condition_var } = t.term in
-  let (| ex_inv, inv_typing |) =
-    check_vprop (push_context "invariant" (term_range inv) g) 
-                (tm_exists_sl u0 { binder_ppname=condition_var; binder_ty=tm_bool } inv)
-  in
-  if RU.debug_at_level (fstar_env g) "inference"
-  then (
-    T.print (Printf.sprintf "Checking precondition of while loop: %s\n" (P.term_to_string ex_inv))
-  );
-  match Framing.check_frameable pre_typing ex_inv with
-  | Inr f -> T.raise (Framing_failure f)
-  | Inl framing_token ->
-    match ex_inv.t with
-    | Tm_ExistsSL u {binder_ppname=nm; binder_ty=ty} inv ->
-      if not (eq_tm ty tm_bool) ||
-         not (eq_univ u u0)
-      then fail g (Some nm.range) "While loop invariant exists but its witness type is not bool"
-      else begin
-        let while_cond_comp_typing = while_cond_comp_typing u nm ty inv inv_typing in
-        let (| res_typing, cond_pre_typing, x, post_typing |) =
-            Metatheory.(st_comp_typing_inversion (comp_typing_inversion while_cond_comp_typing))
-        in
-        let while_cond_hint
-          : post_hint_for_env g
-          = post_hint_from_comp_typing while_cond_comp_typing
-        in
-        let (| cond, cond_comp, cond_typing |) =
-          check' allow_inst
-                 (push_context "while condition" cond.range g)
-                 cond
-                 (comp_pre (comp_while_cond nm inv))
-                 cond_pre_typing
-                 (Some while_cond_hint)
-                 frame_pre
-        in
-        if eq_comp cond_comp (comp_while_cond nm inv)
-        then begin
-          let while_body_comp_typing = while_body_comp_typing u nm ty inv inv_typing in
-          let (| res_typing, body_pre_typing, x, post_typing |) = 
-              Metatheory.(st_comp_typing_inversion (comp_typing_inversion while_body_comp_typing))
-          in
-          let while_post_hint
-            : post_hint_for_env g
-            = post_hint_from_comp_typing while_body_comp_typing
-          in
-          let (| body, body_comp, body_typing |) =
-              check' allow_inst
-                     (push_context "while body" body.range g)
-                     body
-                     (comp_pre (comp_while_body nm inv))
-                     body_pre_typing
-                     (Some while_post_hint)
-                     frame_pre
-          in
-          if eq_comp body_comp (comp_while_body nm inv)
-          then let d = T_While g inv cond body inv_typing cond_typing body_typing in
-               let (| c, st_d |) = Framing.apply_frame pre_typing d framing_token in
-               repack (| c, st_d |) post_hint
-          else 
-            fail g None
-              (Printf.sprintf "Could not prove the inferred type of the while body matches the annotation\n\
-                                     Inferred type = %s\n\
-                                     Annotated type = %s\n"
-                                     (P.comp_to_string body_comp)
-                                     (P.comp_to_string (comp_while_body nm inv)))
-      end
-      else fail g None 
-(Printf.sprintf "Could not prove that the inferred type of the while condition matches the annotation\n\
-                                 Inferred type = %s\n\
-                                 Annotated type = %s\n"
-                                 (P.comp_to_string cond_comp)
-                                 (P.comp_to_string (comp_while_cond nm inv)))
-                end
-     | _ -> fail g None "Typechecked invariant is not an exists"
+// #push-options "--fuel 0 --ifuel 2 --z3rlimit_factor 10 --split_queries no --query_stats"
+// let check_while
+//   (allow_inst:bool)
+//   (g:env)
+//   (t:st_term{Tm_While? t.term})
+//   (pre:term)
+//   (pre_typing:tot_typing g pre tm_vprop)
+//   (post_hint:post_hint_opt g)
+//   (frame_pre:bool)
+//   (check':bool -> check_t)
+//   : T.Tac (checker_result_t g pre post_hint frame_pre) =
+//   if not frame_pre
+//   then T.fail "check_while, frame_pre is false, bailing";
+//   let g = push_context "while loop" t.range g in
+//   let Tm_While { invariant=inv; condition=cond; body; condition_var } = t.term in
+//   let (| ex_inv, inv_typing |) =
+//     check_vprop (push_context "invariant" (term_range inv) g) 
+//                 (tm_exists_sl u0 { binder_ppname=condition_var; binder_ty=tm_bool } inv)
+//   in
+//   if RU.debug_at_level (fstar_env g) "inference"
+//   then (
+//     T.print (Printf.sprintf "Checking precondition of while loop: %s\n" (P.term_to_string ex_inv))
+//   );
+//   match Framing.check_frameable pre_typing ex_inv with
+//   | Inr f -> T.raise (Framing_failure f)
+//   | Inl framing_token ->
+//     match ex_inv.t with
+//     | Tm_ExistsSL u {binder_ppname=nm; binder_ty=ty} inv ->
+//       if not (eq_tm ty tm_bool) ||
+//          not (eq_univ u u0)
+//       then fail g (Some nm.range) "While loop invariant exists but its witness type is not bool"
+//       else begin
+//         let while_cond_comp_typing = while_cond_comp_typing u nm ty inv inv_typing in
+//         let (| res_typing, cond_pre_typing, x, post_typing |) =
+//             Metatheory.(st_comp_typing_inversion (comp_typing_inversion while_cond_comp_typing))
+//         in
+//         let while_cond_hint
+//           : post_hint_for_env g
+//           = post_hint_from_comp_typing while_cond_comp_typing
+//         in
+//         let (| cond, cond_comp, cond_typing |) =
+//           check' allow_inst
+//                  (push_context "while condition" cond.range g)
+//                  cond
+//                  (comp_pre (comp_while_cond nm inv))
+//                  cond_pre_typing
+//                  (Some while_cond_hint)
+//                  frame_pre
+//         in
+//         if eq_comp cond_comp (comp_while_cond nm inv)
+//         then begin
+//           let while_body_comp_typing = while_body_comp_typing u nm ty inv inv_typing in
+//           let (| res_typing, body_pre_typing, x, post_typing |) = 
+//               Metatheory.(st_comp_typing_inversion (comp_typing_inversion while_body_comp_typing))
+//           in
+//           let while_post_hint
+//             : post_hint_for_env g
+//             = post_hint_from_comp_typing while_body_comp_typing
+//           in
+//           let (| body, body_comp, body_typing |) =
+//               check' allow_inst
+//                      (push_context "while body" body.range g)
+//                      body
+//                      (comp_pre (comp_while_body nm inv))
+//                      body_pre_typing
+//                      (Some while_post_hint)
+//                      frame_pre
+//           in
+//           if eq_comp body_comp (comp_while_body nm inv)
+//           then let d = T_While g inv cond body inv_typing cond_typing body_typing in
+//                let (| c, st_d |) = Framing.apply_frame pre_typing d framing_token in
+//                repack (| c, st_d |) post_hint
+//           else 
+//             fail g None
+//               (Printf.sprintf "Could not prove the inferred type of the while body matches the annotation\n\
+//                                      Inferred type = %s\n\
+//                                      Annotated type = %s\n"
+//                                      (P.comp_to_string body_comp)
+//                                      (P.comp_to_string (comp_while_body nm inv)))
+//       end
+//       else fail g None 
+// (Printf.sprintf "Could not prove that the inferred type of the while condition matches the annotation\n\
+//                                  Inferred type = %s\n\
+//                                  Annotated type = %s\n"
+//                                  (P.comp_to_string cond_comp)
+//                                  (P.comp_to_string (comp_while_cond nm inv)))
+//                 end
+//      | _ -> fail g None "Typechecked invariant is not an exists"
